Minor

theories/approx.v
@@ -1,4 +1,5 @@
-Require Export imports.
+Require Export imports typing.
+Require Import Unicoq.Unicoq.
 
 Inductive Skel : Set :=
 | SK_Star : Skel
@@ -9,11 +10,31 @@ Inductive Cls : Set :=
 | C_Type : Skel -> Cls
 | C_Term : Cls.
 
+Definition EBasis := list Cls.
+
+Inductive ELookup : nat -> EBasis -> Cls -> Prop :=
+| EHere c Σ : ELookup 0 (c :: Σ) c
+| EThere n c0 c1 Σ : ELookup n Σ c0 ->
+                     ELookup (S n) (c1::Σ) c0.
+
+(* Inductive HasCl Σ : Term -> Cls -> Prop := *)
+(* | C_Sort : HasCl Σ (ISort Star) (C_Kind SK_Star) *)
+(* | C_Var i c : ELookup i Σ c -> HasCl Σ (VarTm i) . *)
+(* | *)
+
+Definition down_cls c :=
+  match c with
+  | C_Kind sk => C_Type sk
+  | C_Type sk => C_Term
+  | _ => C_Term
+  end.
+
+
 Fixpoint cl_term Σ a : Cls :=
   match a with
   | ISort _ => C_Kind SK_Star
   | VarTm i => match nth_error Σ i with
-              | Some (C_Kind sk) => C_Type sk
+              | Some c => down_cls c
               | _ => C_Term
               end
   | Abs A a => match cl_term Σ A , cl_term (cl_term Σ A :: Σ) a with
@@ -31,3 +52,52 @@ Fixpoint cl_term Σ a : Cls :=
              | _, c => c
              end
   end.
+
+Inductive loose_eqc : Cls -> Cls -> Prop :=
+| L_Kind s :
+  loose_eqc (C_Kind s) (C_Kind s)
+| L_Type s1 s2 :
+  loose_eqc (C_Type s1) (C_Type s2)
+| L_Term :
+  loose_eqc C_Term C_Term.
+
+Definition adj_cls c0 c1 :=
+  match c0, c1 with
+  | C_Type _, C_Kind _ => true
+  | C_Term, C_Type _ => true
+  | _, _ => false
+  end.
+
+Fixpoint cl_basis Γ :=
+  match Γ with
+  | nil => nil
+  | A :: Γ => cl_term (cl_basis Γ) A :: cl_basis Γ
+  end.
+
+Inductive Kind_Or_Else a : Cls ->  Prop :=
+| KoE_Kind sk : Kind_Or_Else a (C_Kind sk)
+| KoE_Else : Kind_Or_Else a a.
+
+Lemma Kind_Or_ElseP a :
+  Kind_Or_Else a a.
+Proof. hauto lq:on inv:Cls ctrs:Kind_Or_Else. Qed.
+
+Lemma cl_term_sound Γ a A :
+  Γ ⊢ a ∈ A ->
+  forall s, Γ ⊢ A ∈ ISort s ->
+  let Σ := cl_basis Γ in
+  adj_cls (cl_term Σ a) (cl_term Σ A).
+Proof.
+  move => h /=. elim : Γ a A / h.
+  (* Easy *)
+  - simpl.
+    admit.
+  (* Contradiction *)
+  - simpl.
+    admit.
+  (*  *)
+  - move => Γ A s1 a B s2 hA ihA ha iha hB ihB s h /=.
+    move E : (cl_term (cl_basis Γ) A) => c0.
+    case : (Kind_Or_ElseP c0) E.
+    + admit.
+    + case :
